updated proofs to use LM_Fair instead of LM

fairness/heap_lang/em_lm_heap_lang.v
@@ -1,18 +1,30 @@
-From trillium.fairness.heap_lang Require Import heap_lang_defs em_lm.
+From trillium.fairness.heap_lang Require Import heap_lang_defs em_lm. 
+From trillium.fairness Require Import lm_fair lm_fair_traces. 
 
 
 Section LM_EM_HL.
-  Context `{LM: LiveModel (locale heap_lang) M LSI}. 
+  Context `{LM: LiveModel (locale heap_lang) M LSI}.
+  (* Context {LF: LMFairPre LM}. *)
+  Context {LF': LMFairPre' LM}.
 
-  Definition LM_EM_HL: ExecutionModel heap_lang LM :=
+  Local Instance LF: LMFairPre LM.
+  esplit; apply _.
+  Defined.   
+
+  Definition LM_EM_HL: ExecutionModel heap_lang (fair_model_model LM_Fair) :=
     LM_EM (LM := LM) 0%nat ltac:(done).
 
-  Global Instance LM_EM_fairPre `{hGS: @heapGpreS Σ LM LM_EM_HL}:
-    fairnessGpreS LM Σ.
-  Proof. apply hGS. Defined. 
+  (* TODO: how to avoid specifying instances of EqDec and Cnt? *)
+  Global Instance LM_EM_fairPre {Σ} {hGS: @heapGpreS Σ _ LM_EM_HL}:
+    (* fairnessGpreS LM Σ. *)
+    fairnessGpreS LM Σ. 
+  Proof.
+    apply hGS.
+  Qed.
 
-(* TODO: get rid of it*)
-  Global Instance LM_EM_fair `{hGS: @heapGS Σ LM LM_EM_HL}:
+  (* TODO: get rid of it*)
+  Global Instance LM_EM_fair `{hGS: @heapGS Σ _ LM_EM_HL}:
+    (* fairnessGS LM Σ. *)
     fairnessGS LM Σ.
   Proof. apply hGS. Defined.
 
