fairness/actual_resources_interface.v
@@ -1,21 +1,26 @@
 From iris.algebra Require Import auth gmap gset excl.
 From iris.proofmode Require Import tactics.
-From trillium.fairness Require Import fairness fuel resources actual_resources heap_lang_defs em_lm em_lm_heap_lang pmp_lifting.
+From trillium.fairness Require Import fairness fuel resources actual_resources heap_lang_defs em_lm em_lm_heap_lang pmp_lifting lm_fair lm_fair_traces.
 
 
 Section ActualOwnershipInterface. 
   Context `{LM: LiveModel (locale heap_lang) M LSI_True}.
   Context {Σ : gFunctors}.
   Context {fG: fairnessGS LM Σ}.
-  Context`{invGS_gen HasNoLc Σ}. 
+  Context {LF': LMFairPre' LM}. 
+  Context`{invGS_gen HasNoLc Σ}.
+
+  Local Instance LF: LMFairPre LM.
+  esplit; apply _.
+  Defined. 
 
   (* TODO: get rid of mim_* lemmas inside of actual_resources *)
   (* TODO: get rid of excessive shelved goals
      (could be solved by new implementation of LiveState) *)
   Lemma ActualOwnershipPartial:
-    ⊢ PartialModelPredicates ∅ (EM := @LM_EM_HL _ _ LM) (iLM := LM) (PMPP := ActualOwnershipPartialPre) (eGS := fG). 
+    ⊢ PartialModelPredicates ∅ (EM := @LM_EM_HL _ _ _ LF') (iLM := LM) (PMPP := ActualOwnershipPartialPre) (eGS := fG). 
   Proof.
-    iIntros. iApply (Build_PartialModelPredicates (EM := @LM_EM_HL _ _ LM)). 
+    iIntros. iApply (Build_PartialModelPredicates (EM := @LM_EM_HL _ _ _ LF')). 
     iModIntro. repeat iSplitL.
     - iIntros (???????) "FUELS MSI". simpl in *.
       iDestruct "MSI" as "[LM_MSI %TR]".
@@ -27,7 +32,7 @@ Section ActualOwnershipInterface.
       + remember (trace_last auxtr) as δ1. 
         pose proof (tids_restrict_smaller _ _ TR) as SM.
         repeat split; eauto.
-        * done.
+        * eexists. split; [apply STEPM| ]. done. 
         * eapply tids_smaller_restrict_mapping; eauto.
           simpl. erewrite (maps_inverse_match_uniq1 (ls_mapping δ2)).
           3: { eapply (mim_fuel_helper _ ∅); eauto.
@@ -72,21 +77,21 @@ Section ActualOwnershipInterface.
           destruct POOL as (?&?&?).
           exists x, efork. done.
       + repeat split; eauto.
-        * done.
-        * eapply tids_smaller_fork_step; eauto.
-          ** by rewrite -LAST.
-          ** simpl. erewrite (maps_inverse_match_uniq1 (ls_mapping δ2)).
-             3: { eapply mim_helper_fork_step.
-                  6: eapply (ls_mapping_tmap_corr δ1).
-                  all: eauto.
-                  rewrite dom_fmap_L in Hxdom.
-                  apply elem_of_subseteq. intros.
-                  apply Hxdom in H0.
-                  apply elem_of_dom. eauto. }
-             { eauto. }
-             rewrite -TMAP'. apply ls_mapping_tmap_corr.
-          ** destruct POOL as (?&?&?).
-             exists x, efork. done.
+        { eexists; split; [apply STEPM| ]; done. } 
+        eapply tids_smaller_fork_step; eauto.
+        * by rewrite -LAST.
+        * simpl. erewrite (maps_inverse_match_uniq1 (ls_mapping δ2)).
+          3: { eapply mim_helper_fork_step.
+               6: eapply (ls_mapping_tmap_corr δ1).
+               all: eauto.
+               rewrite dom_fmap_L in Hxdom.
+               apply elem_of_subseteq. intros.
+               apply Hxdom in H0.
+               apply elem_of_dom. eauto. }
+          { eauto. }
+          rewrite -TMAP'. apply ls_mapping_tmap_corr.
+        * destruct POOL as (?&?&?).
+          exists x, efork. done.
     - iIntros "* FUELS ST MSI FR". simpl in *.
       iDestruct "MSI" as "[LM_MSI %TR]".
       pose proof (tids_restrict_smaller _ _ TR) as SM.
@@ -100,8 +105,8 @@ Section ActualOwnershipInterface.
       iMod (actual_update_step_still_alive with "FUELS ST LM_MSI FR") as (?) "(%STEPM & FUELS & ST & LM_MSI & FR & %TMAP2)"; eauto. 
       iModIntro. do 2 iExists _. iFrame. iPureIntro. split.
       + repeat split; eauto.
-        2: by rewrite LAST2; eauto.
-        { done. }
+        (* 2: by rewrite LAST2; eauto. *)
+        { rewrite LAST2. eexists; split; [apply STEPM| ]. done. }  
         eapply tids_smaller_model_step; eauto.
         do 2 eexists.
         erewrite (maps_inverse_match_uniq1).
